Impl/CoordinationModel.i.dfy
@@ -1,0 +1,363 @@
+include "SyncModel.i.dfy"
+include "CommitterCommitModel.i.dfy"
+include "CommitterInitModel.i.dfy"
+
+module CoordinatorModel {
+  import opened StateModel
+  import opened Options
+  import CommitterModel
+  import IOModel
+  import SyncModel
+  import CommitterCommitModel
+  import CommitterInitModel
+  import opened InterpretationDiskOps
+  import opened ViewOp
+  import opened NativeTypes
+  import DiskLayout
+
+  lemma jcNoOp(k: Constants, s: Variables, s': Variables, vop: VOp)
+  requires CommitterModel.WF(s.jc)
+  requires s.jc == s'.jc
+  requires vop.StatesInternalOp? || vop.JournalInternalOp?
+      || (vop.AdvanceOp? && vop.uiop.NoOp?)
+  ensures JC.Next(Ik(k).jc, CommitterModel.I(s.jc), CommitterModel.I(s'.jc),
+      JournalDisk.NoDiskOp, vop);
+  {
+    assert JC.NoOp(Ik(k).jc, CommitterModel.I(s.jc), CommitterModel.I(s'.jc),
+        JournalDisk.NoDiskOp, vop);
+    assert JC.NextStep(Ik(k).jc, CommitterModel.I(s.jc), CommitterModel.I(s'.jc),
+        JournalDisk.NoDiskOp, vop, JC.NoOpStep);
+  }
+
+  lemma bcNoOp(k: Constants, s: Variables, s': Variables, vop: VOp)
+  requires WFBCVars(s.bc)
+  requires s.bc == s'.bc
+  requires vop.StatesInternalOp? || vop.JournalInternalOp?
+      || vop.PushSyncOp? || vop.PopSyncOp?
+  ensures BBC.Next(Ik(k).bc, IBlockCache(s.bc), IBlockCache(s'.bc),
+      BlockDisk.NoDiskOp, vop);
+  {
+    assert BC.NoOp(Ik(k).bc, IBlockCache(s.bc), IBlockCache(s'.bc),
+        BlockDisk.NoDiskOp, vop);
+    assert BC.NextStep(Ik(k).bc, IBlockCache(s.bc), IBlockCache(s'.bc),
+        BlockDisk.NoDiskOp, vop, BC.NoOpStep);
+    assert BBC.NextStep(Ik(k).bc, IBlockCache(s.bc), IBlockCache(s'.bc),
+        BlockDisk.NoDiskOp, vop, BBC.BlockCacheMoveStep(BC.NoOpStep));
+  }
+
+  lemma noop(k: Constants, s: Variables)
+  requires WFVars(s)
+  ensures M.Next(Ik(k), IVars(s), IVars(s), UI.NoOp, D.NoDiskOp)
+  {
+    jcNoOp(k, s, s, StatesInternalOp);
+    bcNoOp(k, s, s, StatesInternalOp);
+    assert BJC.NextStep(Ik(k), IVars(s), IVars(s), UI.NoOp, IDiskOp(D.NoDiskOp), StatesInternalOp);
+  }
+
+  function {:opaque} pushSync(k: Constants, s: Variables)
+      : (Variables, uint64)
+  requires WFVars(s)
+  {
+    var (jc', id) := CommitterCommitModel.pushSync(k, s.jc);
+    var s' := s.(jc := jc');
+    (s', id)
+  }
+
+  lemma pushSyncCorrect(k: Constants, s: Variables)
+  requires Inv(k, s)
+  ensures var (s', id) := pushSync(k, s);
+    && WFVars(s')
+    && M.Next(Ik(k), IVars(s), IVars(s'),
+       if id == 0 then UI.NoOp else UI.PushSyncOp(id as int),
+       D.NoDiskOp)
+  {
+    reveal_pushSync();
+    var (s', id) := pushSync(k, s);
+    CommitterCommitModel.pushSyncCorrect(k, s.jc);
+
+    var uiop := if id == 0 then UI.NoOp else UI.PushSyncOp(id as int);
+    var vop := if id == 0 then JournalInternalOp else PushSyncOp(id as int);
+    bcNoOp(k, s, s', vop);
+    assert BJC.NextStep(Ik(k), IVars(s), IVars(s'), uiop,
+       BJD.DiskOp(BlockDisk.NoDiskOp, JournalDisk.NoDiskOp),
+       vop);
+    assert BJC.Next(Ik(k), IVars(s), IVars(s'), uiop,
+       BJD.DiskOp(BlockDisk.NoDiskOp, JournalDisk.NoDiskOp));
+    assert M.Next(Ik(k), IVars(s), IVars(s'),
+       if id == 0 then UI.NoOp else UI.PushSyncOp(id as int),
+       D.NoDiskOp);
+  }
+
+  function {:opaque} receiveLoc(k: Constants, s: BCVariables, loc: DiskLayout.Location) : (s': BCVariables)
+  {
+    LoadingIndirectionTable(loc, None)
+  }
+
+  lemma receiveLocCorrect(k: Constants, s: BCVariables, loc: DiskLayout.Location)
+  requires BCInv(k, s)
+  requires DiskLayout.ValidIndirectionTableLocation(loc)
+  requires s.Unready?
+  ensures var s' := receiveLoc(k, s, loc);
+    && WFBCVars(s')
+    && BBC.Next(Ik(k).bc, IBlockCache(s), IBlockCache(s'), BlockDisk.NoDiskOp, SendPersistentLocOp(loc))
+  {
+    reveal_receiveLoc();
+    var s' := receiveLoc(k, s, loc);
+    assert BC.ReceiveLoc(Ik(k).bc, IBlockCache(s), IBlockCache(s'), BlockDisk.NoDiskOp, SendPersistentLocOp(loc));
+    assert BC.NextStep(Ik(k).bc, IBlockCache(s), IBlockCache(s'), BlockDisk.NoDiskOp, SendPersistentLocOp(loc), BC.ReceiveLocStep);
+    assert BBC.NextStep(Ik(k).bc, IBlockCache(s), IBlockCache(s'), BlockDisk.NoDiskOp, SendPersistentLocOp(loc), BBC.BlockCacheMoveStep(BC.ReceiveLocStep));
+  }
+
+  function {:opaque} initialization(k: Constants, s: Variables, io: IO)
+      : (Variables, IO)
+  requires Inv(k, s)
+  requires io.IOInit?
+  {
+    if s.jc.status.StatusLoadingSuperblock? then (
+      if s.jc.superblock1.SuperblockSuccess?
+          && s.jc.superblock2.SuperblockSuccess? then (
+        var cm' := CommitterInitModel.FinishLoadingSuperblockPhase(k, s.jc);
+        var bc' := receiveLoc(
+            k, s.bc, cm'.superblock.indirectionTableLoc);
+        var s' := s.(jc := cm').(bc := bc');
+        (s', io)
+      ) else if s.jc.superblock1Read.None?
+          && s.jc.superblock1.SuperblockUnfinished? then (
+        var (cm', io') := CommitterInitModel.PageInSuperblockReq(k, s.jc, io, 0);
+        var s' := s.(jc := cm');
+        (s', io')
+      ) else if s.jc.superblock2Read.None?
+          && s.jc.superblock2.SuperblockUnfinished? then (
+        var (cm', io') := CommitterInitModel.PageInSuperblockReq(k, s.jc, io, 1);
+        var s' := s.(jc := cm');
+        (s', io')
+      ) else (
+        (s, io)
+      )
+    ) else if s.jc.status.StatusLoadingOther? then (
+      var cm' := CommitterInitModel.FinishLoadingOtherPhase(k, s.jc);
+      var s' := s.(jc := cm');
+      (s', io)
+    ) else if s.bc.LoadingIndirectionTable? &&
+        s.bc.indirectionTableRead.None? then (
+      var (bc', io') := IOModel.PageInIndirectionTableReq(k, s.bc, io);
+      var s' := s.(bc := bc');
+      (s', io')
+    ) else (
+      (s, io)
+    )
+  }
+
+  lemma initializationCorrect(k: Constants, s: Variables, io: IO)
+  requires Inv(k, s)
+  requires io.IOInit?
+  ensures var (s', io') := initialization(k, s, io);
+    && WFVars(s')
+    && M.Next(Ik(k), IVars(s), IVars(s'), UI.NoOp, diskOp(io'))
+  {
+    var (s', io') := initialization(k, s, io);
+    reveal_initialization();
+    if s.jc.status.StatusLoadingSuperblock? {
+      if s.jc.superblock1.SuperblockSuccess?  && s.jc.superblock2.SuperblockSuccess? {
+        CommitterInitModel.FinishLoadingSuperblockPhaseCorrect(k, s.jc);
+        var cm' := CommitterInitModel.FinishLoadingSuperblockPhase(k, s.jc);
+        receiveLocCorrect(k, s.bc, cm'.superblock.indirectionTableLoc);
+        var bc' := receiveLoc(
+            k, s.bc, cm'.superblock.indirectionTableLoc);
+        var s' := s.(jc := cm').(bc := bc');
+        assert BJC.NextStep(Ik(k), IVars(s), IVars(s'), UI.NoOp, IDiskOp(diskOp(io')), SendPersistentLocOp(cm'.superblock.indirectionTableLoc));
+        assert BJC.Next(Ik(k), IVars(s), IVars(s'), UI.NoOp, IDiskOp(diskOp(io')));
+        assert M.Next(Ik(k), IVars(s), IVars(s'), UI.NoOp, diskOp(io'));
+      } else if s.jc.superblock1Read.None?  && s.jc.superblock1.SuperblockUnfinished? {
+        CommitterInitModel.PageInSuperblockReqCorrect(k, s.jc, io, 0);
+        bcNoOp(k, s, s', JournalInternalOp);
+        assert BJC.NextStep(Ik(k), IVars(s), IVars(s'), UI.NoOp, IDiskOp(diskOp(io')), JournalInternalOp);
+        assert BJC.Next(Ik(k), IVars(s), IVars(s'), UI.NoOp, IDiskOp(diskOp(io')));
+        assert M.Next(Ik(k), IVars(s), IVars(s'), UI.NoOp, diskOp(io'));
+      } else if s.jc.superblock2Read.None?  && s.jc.superblock2.SuperblockUnfinished? {
+        CommitterInitModel.PageInSuperblockReqCorrect(k, s.jc, io, 1);
+        bcNoOp(k, s, s', JournalInternalOp);
+        assert BJC.NextStep(Ik(k), IVars(s), IVars(s'), UI.NoOp, IDiskOp(diskOp(io')), JournalInternalOp);
+        assert BJC.Next(Ik(k), IVars(s), IVars(s'), UI.NoOp, IDiskOp(diskOp(io')));
+        assert M.Next(Ik(k), IVars(s), IVars(s'), UI.NoOp, diskOp(io'));
+      } else {
+        noop(k, s);
+      }
+    } else if s.jc.status.StatusLoadingOther? {
+      CommitterInitModel.FinishLoadingOtherPhaseCorrect(k, s.jc);
+      bcNoOp(k, s, s', JournalInternalOp);
+      assert BJC.NextStep(Ik(k), IVars(s), IVars(s'), UI.NoOp, IDiskOp(diskOp(io')), JournalInternalOp);
+      assert BJC.Next(Ik(k), IVars(s), IVars(s'), UI.NoOp, IDiskOp(diskOp(io')));
+      assert M.Next(Ik(k), IVars(s), IVars(s'), UI.NoOp, diskOp(io'));
+    } else if s.bc.LoadingIndirectionTable? &&
+        s.bc.indirectionTableRead.None? {
+      IOModel.PageInIndirectionTableReqCorrect(k, s.bc, io);
+      jcNoOp(k, s, s', StatesInternalOp);
+      assert BJC.NextStep(Ik(k), IVars(s), IVars(s'), UI.NoOp, IDiskOp(diskOp(io')), StatesInternalOp);
+      assert BJC.Next(Ik(k), IVars(s), IVars(s'), UI.NoOp, IDiskOp(diskOp(io')));
+      assert M.Next(Ik(k), IVars(s), IVars(s'), UI.NoOp, diskOp(io'));
+    } else {
+      noop(k, s);
+    }
+  }
+
+  predicate {:opaque} popSync(
+      k: Constants, s: Variables, io: IO, id: uint64, graphSync: bool,
+      s': Variables, io': IO, success: bool)
+  requires Inv(k, s)
+  requires io.IOInit?
+  {
+    if id in s.jc.syncReqs.contents && s.jc.syncReqs.contents[id] == JC.State1 then (
+      var jc' := CommitterCommitModel.popSync(k, s.jc, id);
+      && s' == s.(jc := jc')
+      && io' == io
+      && success == true
+    ) else if !s.bc.Ready? || !s.jc.status.StatusReady? then (
+      && (s', io') == initialization(k, s, io)
+      && success == false
+    ) else if !CommitterInitModel.isReplayEmpty(s.jc) then (
+      && s' == s
+      && io' == io
+      && success == false
+    ) else if s.jc.isFrozen then (
+      if s.jc.frozenLoc.Some? then (
+        && CommitterCommitModel.tryAdvanceLocation(k, s.jc, io, s'.jc, io')
+        && s.bc == s'.bc
+        && success == false
+      ) else (
+        exists froze ::
+          && SyncModel.sync(k, s.bc, io, s'.bc, io', froze)
+          && s.jc == s'.jc
+          && success == false
+      )
+    ) else if s.jc.superblockWrite.Some? then (
+      && s' == s
+      && io' == io
+      && success == false
+    ) else (
+      if graphSync then (
+        exists froze ::
+          && SyncModel.sync(k, s.bc, io, s'.bc, io', froze)
+          && (froze ==> s'.jc == CommitterCommitModel.freeze(k, s.jc))
+          && (!froze ==> s'.jc == s.jc)
+          && success == false
+      ) else (
+        && CommitterCommitModel.tryAdvanceLog(k, s.jc, io, s'.jc, io')
+        && s.bc == s'.bc
+        && success == false
+      )
+    )
+  }
+
+  lemma popSyncCorrect(
+      k: Constants, s: Variables, io: IO, id: uint64, graphSync: bool,
+      s': Variables, io': IO, success: bool)
+  requires Inv(k, s)
+  requires io.IOInit?
+  requires popSync(k, s, io, id, graphSync, s', io', success)
+
+  ensures WFVars(s')
+  ensures M.Next(Ik(k), IVars(s), IVars(s'),
+        if success then UI.PopSyncOp(id as int) else UI.NoOp,
+        diskOp(io'))
+  {
+    reveal_popSync();
+    CommitterInitModel.reveal_isReplayEmpty();
+    if id in s.jc.syncReqs.contents && s.jc.syncReqs.contents[id] == JC.State1 {
+      CommitterCommitModel.popSyncCorrect(k, s.jc, id);
+
+      var uiop := if success then UI.PopSyncOp(id as int) else UI.NoOp;
+      var vop := if success then PopSyncOp(id as int) else JournalInternalOp;
+      bcNoOp(k, s, s', vop);
+      assert BJC.NextStep(Ik(k), IVars(s), IVars(s'), uiop, IDiskOp(diskOp(io')), vop);
+      assert BJC.Next(Ik(k), IVars(s), IVars(s'), uiop, IDiskOp(diskOp(io')));
+      assert M.Next(Ik(k), IVars(s), IVars(s'), uiop, diskOp(io'));
+
+    } else if !s.bc.Ready? || !s.jc.status.StatusReady? {
+      initializationCorrect(k, s, io);
+      assert M.Next(Ik(k), IVars(s), IVars(s'), UI.NoOp, diskOp(io'));
+    } else if !CommitterInitModel.isReplayEmpty(s.jc) {
+      noop(k, s);
+    } else if s.jc.isFrozen {
+      if s.jc.frozenLoc.Some? {
+        CommitterCommitModel.tryAdvanceLocationCorrect(k, s.jc, io, s'.jc, io');
+
+        var uiop := UI.NoOp;
+        var vop := JournalInternalOp;
+        bcNoOp(k, s, s', vop);
+        assert BJC.NextStep(Ik(k), IVars(s), IVars(s'), uiop, IDiskOp(diskOp(io')), vop);
+        assert BJC.Next(Ik(k), IVars(s), IVars(s'), uiop, IDiskOp(diskOp(io')));
+        assert M.Next(Ik(k), IVars(s), IVars(s'), uiop, diskOp(io'));
+      } else {
+        var froze :|
+          && SyncModel.sync(k, s.bc, io, s'.bc, io', froze)
+          && s.jc == s'.jc
+          && success == false;
+        SyncModel.syncCorrect(k, s.bc, io, s'.bc, io', froze);
+
+        assert !froze;
+
+        var uiop := UI.NoOp;
+        if BBC.Next(Ik(k).bc, IBlockCache(s.bc), IBlockCache(s'.bc), IDiskOp(diskOp(io')).bdop, StatesInternalOp) {
+          var vop := StatesInternalOp;
+          jcNoOp(k, s, s', vop);
+          assert BJC.NextStep(Ik(k), IVars(s), IVars(s'), uiop, IDiskOp(diskOp(io')), vop);
+          assert BJC.Next(Ik(k), IVars(s), IVars(s'), uiop, IDiskOp(diskOp(io')));
+          assert M.Next(Ik(k), IVars(s), IVars(s'), UI.NoOp, diskOp(io'));
+        } else {
+          var vop := AdvanceOp(UI.NoOp, false);
+          assert BBC.Next(Ik(k).bc, IBlockCache(s.bc), IBlockCache(s'.bc), IDiskOp(diskOp(io')).bdop, vop);
+          jcNoOp(k, s, s', vop);
+          assert BJC.NextStep(Ik(k), IVars(s), IVars(s'), uiop, IDiskOp(diskOp(io')), vop);
+          assert BJC.Next(Ik(k), IVars(s), IVars(s'), uiop, IDiskOp(diskOp(io')));
+          assert M.Next(Ik(k), IVars(s), IVars(s'), UI.NoOp, diskOp(io'));
+        }
+      }
+    } else if s.jc.superblockWrite.Some? {
+      noop(k, s);
+    } else {
+      if graphSync {
+        var froze :|
+          && SyncModel.sync(k, s.bc, io, s'.bc, io', froze)
+          && (froze ==> s'.jc == CommitterCommitModel.freeze(k, s.jc))
+          && (!froze ==> s'.jc == s.jc)
+          && success == false;
+
+          SyncModel.syncCorrect(k, s.bc, io, s'.bc, io', froze);
+          if froze {
+            CommitterCommitModel.freezeCorrect(k, s.jc);
+            assert BJC.NextStep(Ik(k), IVars(s), IVars(s'), UI.NoOp, IDiskOp(diskOp(io')), FreezeOp);
+            assert BJC.Next(Ik(k), IVars(s), IVars(s'), UI.NoOp, IDiskOp(diskOp(io')));
+            assert M.Next(Ik(k), IVars(s), IVars(s'), UI.NoOp, diskOp(io'));
+          } else {
+            var uiop := UI.NoOp;
+            if BBC.Next(Ik(k).bc, IBlockCache(s.bc), IBlockCache(s'.bc), IDiskOp(diskOp(io')).bdop, StatesInternalOp) {
+              var vop := StatesInternalOp;
+              jcNoOp(k, s, s', vop);
+              assert BJC.NextStep(Ik(k), IVars(s), IVars(s'), uiop, IDiskOp(diskOp(io')), vop);
+              assert BJC.Next(Ik(k), IVars(s), IVars(s'), uiop, IDiskOp(diskOp(io')));
+              assert M.Next(Ik(k), IVars(s), IVars(s'), UI.NoOp, diskOp(io'));
+            } else {
+              var vop := AdvanceOp(UI.NoOp, false);
+              assert BBC.Next(Ik(k).bc, IBlockCache(s.bc), IBlockCache(s'.bc), IDiskOp(diskOp(io')).bdop, vop);
+              jcNoOp(k, s, s', vop);
+              assert BJC.NextStep(Ik(k), IVars(s), IVars(s'), uiop, IDiskOp(diskOp(io')), vop);
+              assert BJC.Next(Ik(k), IVars(s), IVars(s'), uiop, IDiskOp(diskOp(io')));
+              assert M.Next(Ik(k), IVars(s), IVars(s'), UI.NoOp, diskOp(io'));
+            }
+
+            assert M.Next(Ik(k), IVars(s), IVars(s'), UI.NoOp, diskOp(io'));
+          }
+      } else {
+        CommitterCommitModel.tryAdvanceLogCorrect(k, s.jc, io, s'.jc, io');
+
+        var uiop := UI.NoOp;
+        var vop := JournalInternalOp;
+        bcNoOp(k, s, s', vop);
+        assert BJC.NextStep(Ik(k), IVars(s), IVars(s'), uiop, IDiskOp(diskOp(io')), vop);
+        assert BJC.Next(Ik(k), IVars(s), IVars(s'), uiop, IDiskOp(diskOp(io')));
+        assert M.Next(Ik(k), IVars(s), IVars(s'), UI.NoOp, diskOp(io'));
+      }
+    }
+  }
+}
