Impl/HandleReadResponseModel.i.dfy
@@ -1,0 +1,125 @@
+include "IOModel.i.dfy"
+
+module HandleReadResponseModel {
+  import opened NativeTypes
+  import opened StateModel
+  import opened DiskLayout
+  import opened InterpretationDiskOps
+  import opened ViewOp
+  import opened Options
+  import IOModel
+  import CommitterModel
+
+  function {:opaque} readSuperblockResp(
+      k: Constants,
+      cm: CommitterModel.CM,
+      io: IO,
+      which: uint64) : CommitterModel.CM
+  requires diskOp(io).RespReadOp?
+  {
+    var (id, sector) := IOModel.ReadSector(io);
+    var res := (if sector.Some? && sector.value.SectorSuperblock?
+        then JC.SuperblockSuccess(sector.value.superblock)
+        else JC.SuperblockCorruption);
+    if which == 0 then (
+      if Some(id) == cm.superblock1Read then
+        cm.(superblock1 := res)
+          .(superblock1Read := None)
+      else
+        cm
+    ) else (
+      if Some(id) == cm.superblock2Read then
+        cm.(superblock2 := res)
+          .(superblock2Read := None)
+      else
+        cm
+    )
+  }
+
+  lemma readSuperblockRespCorrect(
+      k: Constants,
+      cm: CommitterModel.CM,
+      io: IO,
+      which: uint64)
+  requires CommitterModel.WF(cm)
+  requires ValidDiskOp(diskOp(io))
+  requires diskOp(io).RespReadOp?
+  requires which == 0 || which == 1
+  requires which == 0 ==>
+      LocOfRespRead(diskOp(io).respRead) == Superblock1Location()
+  requires which == 1 ==>
+      LocOfRespRead(diskOp(io).respRead) == Superblock2Location()
+  ensures var cm' := readSuperblockResp(k, cm, io, which);
+    && CommitterModel.WF(cm')
+    && JC.Next(Ik(k).jc,
+        CommitterModel.I(cm),
+        CommitterModel.I(cm'),
+        IDiskOp(diskOp(io)).jdop,
+        JournalInternalOp)
+  {
+    var cm' := readSuperblockResp(k, cm, io, which);
+    reveal_readSuperblockResp();
+    IOModel.ReadSectorCorrect(io);
+    var dop := IDiskOp(diskOp(io)).jdop;
+    assert dop.RespReadSuperblockOp?;
+    assert dop.which == which as int;
+
+    if cm.status.StatusLoadingSuperblock?
+        && (which == 0 ==> Some(dop.id) == cm.superblock1Read)
+        && (which == 1 ==> Some(dop.id) == cm.superblock2Read)
+    {
+      assert JC.PageInSuperblockResp(Ik(k).jc,
+          CommitterModel.I(cm),
+          CommitterModel.I(cm'),
+          dop,
+          JournalInternalOp, which as int);
+      assert JC.NextStep(Ik(k).jc,
+          CommitterModel.I(cm),
+          CommitterModel.I(cm'),
+          dop,
+          JournalInternalOp,
+          JC.PageInSuperblockRespStep(which as int));
+    } else {
+      assert JC.NoOp(Ik(k).jc,
+          CommitterModel.I(cm),
+          CommitterModel.I(cm'),
+          dop,
+          JournalInternalOp);
+      assert JC.NextStep(Ik(k).jc,
+          CommitterModel.I(cm),
+          CommitterModel.I(cm'),
+          dop,
+          JournalInternalOp,
+          JC.NoOpStep);
+    }
+  }
+
+  function readResponse(k: Constants, s: Variables, io: IO)
+      : Variables
+  requires Inv(k, s)
+  requires diskOp(io).RespReadOp?
+  requires |io.respRead.bytes| < 0x1_0000_0000_0000_0000
+  {
+    var loc := DiskLayout.Location(
+        io.respRead.addr,
+        |io.respRead.bytes| as uint64);
+
+    if ValidNodeLocation(loc) then (
+      if s.bc.Ready? then (
+        var bc' := IOModel.PageInNodeResp(k, s.bc, io);
+        s.(bc := bc')
+      ) else (
+        s
+      )
+    ) else if ValidIndirectionTableLocation(loc) then (
+      if s.bc.LoadingIndirectionTable? then (
+        var bc' := IOModel.PageInIndirectionTableResp(k, s.bc, io);
+        s.(bc := bc')
+      ) else (
+        s
+      )
+    ) else (
+      s
+    )
+  }
+}
